Liveness

ironfleet/src/Dafny/Distributed/LockProof/LivenessProof/Defs.i.dfy
@@ -1,14 +1,15 @@
 include "../../Protocol/Lock/RefinementProof/DistributedSystem.i.dfy"
 include "../../Common/Logic/Temporal/LeadsTo.i.dfy"
-include "Assumptions.i.dfy"
+include "../../Common/Framework/EnvironmentSynchrony.s.dfy"
 
 module Lock__LivenessProof__Defs_i {
 
 import opened DistributedSystem_i
 import opened Math__mod_auto_i
 import opened Temporal__LeadsTo_i
-import opened Lock__LivenessProof__Assumptions_i
+import opened EnvironmentSynchrony_s
 
+datatype AssumptionParameters = AssumptionParameters()
 
 //================ Functions ==================
 
@@ -28,12 +29,82 @@ ensures i == |config| - 1 ==> NextNode(i, config) == 0
 //================ Predicates ==================
 
 
+predicate ValidTransferPacket(p:LockPacket, config:Config)
+{
+    p.msg.Transfer?
+ && p.src in config
+ && p.dst in config
+}
+
+predicate UsefulTransfer(p:LockPacket, node:EndPoint, config:Config, ls:LS_State)
+{
+    ValidTransferPacket(p, config)
+ && p.dst == node
+ && node in ls.servers
+ && p.msg.transfer_epoch > ls.servers[node].epoch
+}
+
 
 predicate ValidBehavior(b:Behavior<LS_State>, config:Config) {
     imaptotal(b)
  && LS_Init(b[0], config)
  && forall i :: i >= 0 ==> LS_Next(b[i], b[i+1])
 }
+
+predicate PacketsEventuallyDeliveredForHosts(
+    b:Behavior<LEnvironment<EndPoint, LockMessage>>,
+    i:int,
+    serverAddresses:set<EndPoint>
+    )
+    requires imaptotal(b)
+{
+    forall p {:triger PacketSentBetweenHosts(b[i], p, serverAddresses, serverAddresses)} ::
+        PacketSentBetweenHosts(b[i], p, serverAddresses, serverAddresses) ==>
+        sat(i, next(eventual(PacketDeliveredTemporal(b, p))))
+}
+
+predicate PacketReceived(ls:LS_State, p:LockPacket)
+{
+    ls.environment.nextStep.LEnvStepHostIos?
+ && LIoOpReceive(p) in ls.environment.nextStep.ios
+}
+
+predicate IosStep(ls:LS_State) 
+{
+       ls.environment.nextStep.LEnvStepHostIos?
+    && ls.environment.nextStep.actor in ls.servers
+}
+
+predicate NodeGrantOccursForServer(ls:LS_State, ls':LS_State, node:EndPoint)
+{
+    node in ls.servers
+ && node in ls'.servers
+ && ls.environment.nextStep.LEnvStepHostIos?
+ && node == ls.environment.nextStep.actor
+ && NodeGrant(ls.servers[node], ls'.servers[node], ls.environment.nextStep.ios)
+}
+
+predicate NodeAcceptOccursForServer(ls:LS_State, ls':LS_State, node:EndPoint)
+{
+    node in ls.servers
+ && node in ls'.servers
+ && ls.environment.nextStep.LEnvStepHostIos?
+ && node == ls.environment.nextStep.actor
+ && NodeAccept(ls.servers[node], ls'.servers[node], ls.environment.nextStep.ios)
+}
+
+predicate HoldLockForNode(ls:LS_State, node:EndPoint)
+{
+    node in ls.servers
+ && ls.servers[node].held
+}
+
+predicate HoldLockForNodeWithEpoch(ls:LS_State, node:EndPoint, epoch:int)
+{
+    HoldLockForNode(ls, node)
+ && ls.servers[node].epoch == epoch
+}
+
 
 predicate LockedIthPositionWithEpoch(ls:LS_State, i:int, epoch:int, config:Config) 
 requires |config| > 0
@@ -65,23 +136,150 @@ requires 0 <= i < |config|
 {
     forall j ::
            i < j < |config|
-       ==> sat(t, eventual(LockedIthPositionWithHigherEpochTemporal(b, j, epoch, config)))
+       ==> sat(t, eventual(LockedIthPositionWithEpochTemporal(b, j, epoch + j - i, config)))
 }
 
 predicate NodeGrantPacket(ls:LS_State, i:int, epoch:int, config:Config)
 requires 0 <= i < |config|
 {
-       ls.environment.nextStep.LEnvStepHostIos?
-    && exists p : LockPacket ::
-              LIoOpSend(p) in ls.environment.nextStep.ios
-           && p.src == config[i]
-           && p.dst == config[NextNode(i, config)]
-           && p.msg.Transfer?
-           && p.msg.transfer_epoch == epoch
+    exists p : LockPacket ::
+           p in ls.environment.sentPackets
+        && p.src == config[i]
+        && p.dst == config[NextNode(i, config)]
+        && p.msg.Transfer?
+        && p.msg.transfer_epoch == epoch
+}
+
+predicate TransferSent(ls:LS_State, node:EndPoint, epoch:int)
+{
+    node in ls.servers
+ && ls.environment.nextStep.LEnvStepHostIos?
+ && var actor := ls.environment.nextStep.actor;
+    var ios := ls.environment.nextStep.ios;
+    |ios| == 1
+ && ios[0].LIoOpSend?
+ && var p := ios[0].s;
+    p.msg.Transfer?
+ && p.msg.transfer_epoch == epoch
+}
+
+predicate LargestEpoch(ls:LS_State, epoch:int)
+{
+    forall node ::
+           node in ls.servers
+       ==> ls.servers[node].epoch < epoch
+}
+
+predicate ReceiveStep(ls:LS_State, node:EndPoint)
+{
+    ls.environment.nextStep.LEnvStepHostIos?
+ && node == ls.environment.nextStep.actor
+ && |ls.environment.nextStep.ios| > 0
+ && var ios := ls.environment.nextStep.ios;
+    (ios[0].LIoOpReceive? || ios[0].LIoOpTimeoutReceive?)
 }
 
 //================== Temporals ====================
 
+
+function PacketsEventuallyDeliveredForHostsTemporal(
+    b:Behavior<LEnvironment<EndPoint,LockMessage>>,
+    serverAddresses:set<EndPoint>
+    ) : temporal 
+    requires imaptotal(b)
+    ensures forall i {:trigger sat(i, PacketsEventuallyDeliveredForHostsTemporal(b, serverAddresses))} ::
+        sat(i, PacketsEventuallyDeliveredForHostsTemporal(b, serverAddresses)) <==> 
+        PacketsEventuallyDeliveredForHosts(b, i, serverAddresses)
+{
+    stepmap(imap i :: PacketsEventuallyDeliveredForHosts(b, i, serverAddresses))
+}
+
+function PacketReceivedTemporal(b:Behavior<LS_State>, p:LockPacket) : temporal
+requires imaptotal(b)
+ensures forall i {:trigger sat(i, PacketReceivedTemporal(b, p))} :: sat(i, PacketReceivedTemporal(b, p)) <==> PacketReceived(b[i], p)
+{
+    stepmap(imap i :: PacketReceived(b[i], p))
+}
+
+function PacketDeliveredLeadsToReceived(b:Behavior<LS_State>, p:LockPacket) : temporal
+requires imaptotal(b)
+{
+    imply(
+        PacketDeliveredTemporal(BehaviorToLEnvMap(b), p),
+        next(eventual(PacketReceivedTemporal(b, p))))
+}
+
+function BehaviorToLEnvMap(b:Behavior<LS_State>) : imap<int, LEnvironment<EndPoint, LockMessage>>
+requires imaptotal(b)
+ensures imaptotal(BehaviorToLEnvMap(b))
+ensures forall i {:trigger BehaviorToLEnvMap(b)[i]} :: BehaviorToLEnvMap(b)[i] == b[i].environment
+{
+    imap i :: b[i].environment
+}
+
+function IosStepTemporal(b:Behavior<LS_State>) : temporal
+requires imaptotal(b)
+ensures forall t {:trigger sat(t, IosStepTemporal(b))} ::
+               sat(t, IosStepTemporal(b)) <==> IosStep(b[t])
+{
+    stepmap(imap t :: IosStep(b[t]))
+}
+
+
+function EventuallyIosStepTemporal(b:Behavior<LS_State>) : temporal
+requires imaptotal(b)
+{
+    eventual(IosStepTemporal(b))
+}
+
+function NodeGrantOccursForServerTemporal(b:Behavior<LS_State>, node:EndPoint) : temporal
+requires imaptotal(b)
+ensures forall t {:trigger sat(t, NodeGrantOccursForServerTemporal(b, node))} ::
+               sat(t, NodeGrantOccursForServerTemporal(b, node)) <==> NodeGrantOccursForServer(b[t], b[t+1], node)
+{
+    stepmap(imap t :: NodeGrantOccursForServer(b[t], b[t+1], node))
+}
+
+function NodeAcceptOccursForServerTemporal(b:Behavior<LS_State>, node:EndPoint) : temporal
+requires imaptotal(b)
+ensures forall t {:trigger sat(t, NodeAcceptOccursForServerTemporal(b, node))} ::
+               sat(t, NodeAcceptOccursForServerTemporal(b, node)) <==> NodeAcceptOccursForServer(b[t], b[t+1], node)
+{
+    stepmap(imap t :: NodeAcceptOccursForServer(b[t], b[t+1], node))
+}
+
+function HoldLockForNodeTemporal(b:Behavior<LS_State>, node:EndPoint) : temporal
+requires imaptotal(b)
+ensures forall t {:trigger sat(t, HoldLockForNodeTemporal(b, node))} :: sat(t, HoldLockForNodeTemporal(b, node)) <==> HoldLockForNode(b[t], node)
+{
+    stepmap(imap t :: HoldLockForNode(b[t], node))
+}
+
+function HoldLockForNodeWithEpochTemporal(b:Behavior<LS_State>, node:EndPoint, epoch:int) : temporal
+requires imaptotal(b)
+ensures forall t {:trigger sat(t, HoldLockForNodeWithEpochTemporal(b, node, epoch))} :: sat(t, HoldLockForNodeWithEpochTemporal(b, node, epoch)) <==> HoldLockForNodeWithEpoch(b[t], node, epoch)
+{
+    stepmap(imap t :: HoldLockForNodeWithEpoch(b[t], node, epoch))
+}
+
+
+
+function ActionOccursForServerTemporal(b:Behavior<LS_State>, node:EndPoint) : temporal
+requires imaptotal(b)
+{
+//     and(
+//         imply(HoldLockForNodeWithEpochTemporal(b, node, epoch),
+//               eventual(and(HoldLockForNodeWithEpochTemporal(b, node, epoch),
+//                            NodeGrantOccursForServerTemporal(b, node)))),
+//         imply(not(HoldLockForNodeTemporal(b, node)),
+//               eventual(and(not(HoldLockForNodeTemporal(b,node)),
+//                            NodeAcceptOccursForServerTemporal(b, node)))))
+    and(
+        eventual(
+            NodeGrantOccursForServerTemporal(b, node)),
+        eventual(
+            NodeAcceptOccursForServerTemporal(b, node)))
+}
 
 
 function LockedIthPositionWithEpochTemporal(b:Behavior<LS_State>, i:int, epoch:int, config:Config) : temporal
@@ -114,6 +312,11 @@ ensures forall t {:trigger sat(t, EventuallyLockedForAllAfterTemporal(b, i, epoc
     stepmap(imap t :: EventuallyLockedForAllAfter(b, t, i, epoch, config))
 }
 
+function EpochUpperBound(epoch:int, ub:int) : temporal
+{
+    stepmap(imap i :: epoch < ub)
+}
+
 
 
 function LockedImpliesLockedAtNextPositionTemporal(b:Behavior<LS_State>, i:int, epoch:int, config:Config) : temporal
@@ -121,9 +324,8 @@ requires imaptotal(b)
 requires |config| > 0
 requires 0 <= i < |config| - 1
 {
-    imply(or(LockedIthPositionWithEpochTemporal(b, i, epoch, config),
-               LockedIthPositionWithHigherEpochTemporal(b, i, epoch, config)), 
-            eventual(LockedIthPositionWithHigherEpochTemporal(b, i+1, epoch, config)))
+    imply(LockedIthPositionWithEpochTemporal(b, i, epoch, config),
+            eventual(LockedIthPositionWithEpochTemporal(b, i+1, epoch+1, config)))
 }
 
 
@@ -133,9 +335,7 @@ requires |config| > 0
 requires 0 <= i < |config| - 1
 {
     imply(
-        or(
-            LockedIthPositionWithEpochTemporal(b, i, epoch, config), 
-            LockedIthPositionWithHigherEpochTemporal(b, i, epoch, config)),
+        LockedIthPositionWithEpochTemporal(b, i, epoch, config), 
         EventuallyLockedForAllAfterTemporal(b, i, epoch, config))
 }
 
@@ -144,10 +344,8 @@ requires imaptotal(b)
 requires |config| > 0
 {
     imply(
-        or(
-            LockedIthPositionWithEpochTemporal(b, |config|-1, epoch, config),
-            LockedIthPositionWithHigherEpochTemporal(b, |config|-1, epoch, config)),
-        eventual(LockedIthPositionWithHigherEpochTemporal(b, 0, epoch, config)))
+        LockedIthPositionWithEpochTemporal(b, |config|-1, epoch, config),
+        eventual(LockedIthPositionWithEpochTemporal(b, 0, epoch+1, config)))
 }
 
 
@@ -156,9 +354,8 @@ requires imaptotal(b)
 requires |config| > 0
 requires 0 <= i < |config|
 {
-    imply(or(LockedIthPositionWithEpochTemporal(b, i, epoch, config),
-               LockedIthPositionWithHigherEpochTemporal(b, i, epoch, config)), 
-          eventual(LockedIthPositionWithHigherEpochTemporal(b, NextNode(i, config), epoch, config)))
+    imply(LockedIthPositionWithEpochTemporal(b, i, epoch, config),
+          eventual(LockedIthPositionWithEpochTemporal(b, NextNode(i, config), epoch+1, config)))
 }
 
 
@@ -196,7 +393,31 @@ requires p.dst == config[i]
 requires p.msg.Transfer?
 {
     imply(PacketDeliveredTemporal(BehaviorToLEnvMap(b), p),
-          next(LockedIthPositionWithEpochTemporal(b, i, p.msg.transfer_epoch, config)))
+          next(eventual(LockedIthPositionWithEpochTemporal(b, i, p.msg.transfer_epoch, config))))
 }
+
+function NotHeldUntilAcceptTemporal(b:Behavior<LS_State>, node:EndPoint) : temporal
+requires imaptotal(b)
+{
+        imply(NodeAcceptOccursForServerTemporal(b, node),
+                     not(HoldLockForNodeTemporal(b, node)))
+            
+}
+
+
+function TransferSentTemporal(b:Behavior<LS_State>, node:EndPoint, epoch:int) : temporal
+requires imaptotal(b) 
+ensures forall t {:trigger sat(t, TransferSentTemporal(b, node, epoch))} :: sat(t, TransferSentTemporal(b, node, epoch)) <==> TransferSent(b[t], node, epoch)
+{
+    stepmap(imap t :: TransferSent(b[t], node, epoch))
+}
+
+function ReceiveStepTemporal(b:Behavior<LS_State>, node:EndPoint) : temporal
+requires imaptotal(b)
+ensures forall t {:trigger sat(t, ReceiveStepTemporal(b, node))} :: sat(t, ReceiveStepTemporal(b, node)) <==> ReceiveStep(b[t], node)
+{
+    stepmap(imap t :: ReceiveStep(b[t], node))
+}
+
 
 }
