ironfleet/src/Dafny/Distributed/LockProof/LivenessProof/Invariant.i.dfy
@@ -1,0 +1,22 @@
+include "Defs.i.dfy"
+include "Misc.i.dfy"
+
+
+
+module Lock__LivenessProof__Invariant_i {
+
+import opened Lock__LivenessProof__Defs_i
+import opened Lock__LivenessProof__Misc_i
+
+// TODO
+lemma OnlyOneUsefulTransfer(b:Behavior<LS_State>, t:int, p:LockPacket, p':LockPacket, node:EndPoint, config:Config)
+requires ValidBehavior(b, config)
+requires t >= 0
+requires UsefulTransfer(p, node, config, b[t])
+requires UsefulTransfer(p', node, config, b[t])
+ensures p == p'
+{
+
+}
+
+}
