ironfleet/src/Dafny/Distributed/LockProof/LivenessProof/LockNext.i.dfy
@@ -2,126 +2,383 @@ include "../../../Libraries/Math/mod_auto.i.dfy"
 include "../../Protocol/Lock/RefinementProof/DistributedSystem.i.dfy"
 include "Assumptions.i.dfy"
 include "Defs.i.dfy"
+include "Misc.i.dfy"
+include "Invariant.i.dfy"
 
 module Lock__LivenessProof__LockNext_i {
 
 import opened DistributedSystem_i
 import opened Lock__LivenessProof__Defs_i
 import opened Lock__LivenessProof__Assumptions_i
+import opened Lock__LivenessProof__Misc_i
+import opened Lock__LivenessProof__Invariant_i
 
-
-// TODO
 lemma EventuallyNodeGrant(b:Behavior<LS_State>, i:int, epoch:int, config:Config, asp:AssumptionParameters)
 requires ValidBehavior(b, config)
 requires LivenessAssumptions(b, asp, config)
+requires epoch < 0xFFFF_FFFF_FFFF_FFFF
 requires 0 <= i < |config|
 ensures sat(0, always(LockedImpliesGrantTemporal(b, i, epoch, config)))
 {
+    forall t |
+           t >= 0
+        && sat(t, LockedIthPositionWithEpochTemporal(b, i, epoch, config))
+    ensures sat(t, EventualNodeGrantPacketTemporal(b, i, epoch+1, config))
+    {
+        var p := GetLockPacket(b[t], i, epoch, config);
+        var sendStep := GetSendStep(b, t, p, config);
+        ValidBehaviorServers(b, config);
+        assert b[sendStep].environment.nextStep.LEnvStepHostIos?;
+        var ios := b[sendStep].environment.nextStep.ios;
+        assert p.src == config[i];
+        assert LEnvironment_Next(b[sendStep].environment, b[sendStep+1].environment);
+        assert IsValidLEnvStep(b[sendStep].environment, b[sendStep].environment.nextStep);
+        assert b[sendStep].environment.nextStep.actor == config[i];
+        assert NodeAccept(b[sendStep].servers[config[i]], b[sendStep+1].servers[config[i]], ios);
+        assert b[sendStep+1].servers[config[i]].held;
+        
+        assert sat(sendStep+1, HoldLockForNodeWithEpochTemporal(b, config[i], epoch));
+        reveal_always();
+        reveal_and();
+        reveal_imply();
+        assert sat(sendStep+1, ActionOccursForServerTemporal(b, config[i]));
+        assert sat(sendStep+1, eventual(NodeGrantOccursForServerTemporal(b, config[i])));
+        var grantStep := FirstEventualStep(sendStep+1, NodeGrantOccursForServerTemporal(b, config[i]));
+
+        var k := sendStep + 1;
+        assert b[k].servers[config[i]].held;
+        assert b[k].servers[config[i]].epoch == epoch;
+        while (k < grantStep)
+        invariant sendStep + 1 <= k <= grantStep
+        invariant b[k].servers[config[i]].held
+        invariant b[k].servers[config[i]].epoch == epoch
+        {
+            if (b[k].environment.nextStep.LEnvStepHostIos?
+             && config[i] == b[k].environment.nextStep.actor) {
+                assert !sat(k, NodeGrantOccursForServerTemporal(b, config[i]));
+                ValidBehaviorServers(b, config);
+                assert config[i] in b[k].servers;
+                assert config[i] in b[k+1].servers;
+                assert !NodeGrant(b[k].servers[config[i]], b[k+1].servers[config[i]], b[k].environment.nextStep.ios);
+                assert b[k].servers[config[i]].held;
+            } else {
+                assert b[k].servers[config[i]].held;
+            }
+            k := k + 1;
+        }
+
+        assert b[grantStep].servers[config[i]].held;
+        assert  NodeGrant(b[grantStep].servers[config[i]],
+                          b[grantStep+1].servers[config[i]],
+                          b[grantStep].environment.nextStep.ios);
+        var grantIos := b[grantStep].environment.nextStep.ios;
+        assert |grantIos| == 1;
+        var grantP := grantIos[0].s;
+        assert grantP in b[grantStep+1].environment.sentPackets;
+        assert grantP.src == config[i];
+        NodeConfig(b , config);
+        assert b[grantStep].servers[config[i]].config == config;
+        assert b[grantStep].servers[config[i]].my_index == i;
+        assert grantP.dst == config[NextNode(i, config)];
+        assert grantP.msg.Transfer?;
+        assert grantP.msg.transfer_epoch == epoch+1;
+
+        assert sat(grantStep+1, NodeGrantPacketTemporal(b, i, epoch+1, config));
+        SentPacketsMonotone(b, grantStep+1, i, epoch+1, config);
+
+    }
+    reveal_imply();
+    reveal_always();
 }
 
-// lemma GetEpoch(b:Behavior<LS_State>, t:int, i:int, epoch:int, config:Config) 
-// returns (epoch' : int)
-// requires imaptotal(b)
-// requires 0 <= i < |config|
-// requires sat(t, LockedIthPositionWithHigherEpochTemporal(b, i, epoch, config))
-// ensures epoch' > epoch
-// ensures sat(t, LockedIthPositionWithEpochTemporal(b, i, epoch', config))
-// {
-//     assert LockedIthPositionWithHigherEpoch(b[t], i, epoch, config);
-//     var p, e :|
-//            e > epoch
-//         && p in b[t].environment.sentPackets
-//         && p.src == config[i] 
-//         && p.msg.Locked?
-//         && p.msg.locked_epoch == e;
-//     epoch' := e;
-// }
-
-// lemma GetTransferPacket(b:Behavior<LS_State>, t:int, i:int, epoch:int, config:Config) 
-// returns (p : LockPacket)
-// requires imaptotal(b)
-// requires 0 <= i < |config|
-// requires sat(t, NodeGrantPacketTemporal(b, i, epoch, config))
-// ensures LIoOpSend(p) in b[t].environment.nextStep.ios
-// ensures p.src == config[i]
-// ensures p.dst == config[NextNode(i, config)]
-// ensures p.msg.Transfer?
-// ensures p.msg.transfer_epoch == epoch
-// {
-//     assert NodeGrantPacket(b[t], i, epoch, config);
-//     p :|
-//         LIoOpSend(p) in b[t].environment.nextStep.ios
-//      && p.src == config[i]
-//      && p.dst == config[NextNode(i, config)]
-//      && p.msg.Transfer?
-//      && p.msg.transfer_epoch == epoch;
-// }
-
-// TODO
-lemma TransferDeliveredLeadsToLockedLemma(b:Behavior<LS_State>, p:LockPacket, i:int, config:Config)
+lemma GetEpoch(b:Behavior<LS_State>, t:int, i:int, epoch:int, config:Config) 
+returns (epoch' : int)
 requires imaptotal(b)
-requires ValidBehavior(b, config)
-requires p.msg.Transfer?
 requires 0 <= i < |config|
-requires p.dst == config[i]
-ensures sat(0, always(TransferDeliveredLeadsToLockedTemporal(b, p, i, config)))
+requires sat(t, LockedIthPositionWithHigherEpochTemporal(b, i, epoch, config))
+ensures epoch' > epoch
+ensures sat(t, LockedIthPositionWithEpochTemporal(b, i, epoch', config))
 {
+    assert LockedIthPositionWithHigherEpoch(b[t], i, epoch, config);
+    var p, e :|
+           e > epoch
+        && p in b[t].environment.sentPackets
+        && p.src == config[i] 
+        && p.msg.Locked?
+        && p.msg.locked_epoch == e;
+    epoch' := e;
+}
+
+lemma GetTransferPacket(b:Behavior<LS_State>, t:int, i:int, epoch:int, config:Config) 
+returns (p : LockPacket)
+requires imaptotal(b)
+requires 0 <= i < |config|
+requires sat(t, NodeGrantPacketTemporal(b, i, epoch, config))
+ensures p in b[t].environment.sentPackets
+ensures p.src == config[i]
+ensures p.dst == config[NextNode(i, config)]
+ensures p.msg.Transfer?
+ensures p.msg.transfer_epoch == epoch
+{
+    assert NodeGrantPacket(b[t], i, epoch, config);
+    p :|
+        p in b[t].environment.sentPackets
+     && p.src == config[i]
+     && p.dst == config[NextNode(i, config)]
+     && p.msg.Transfer?
+     && p.msg.transfer_epoch == epoch;
+}
+
+lemma LockedWithEpochToHigherEpoch(b:Behavior<LS_State>, t:int, i:int, epoch:int, epoch':int, config:Config)
+requires imaptotal(b)
+requires 0 <= i < |config|
+requires sat(t, eventual(LockedIthPositionWithEpochTemporal(b, i, epoch, config)))
+requires epoch > epoch'
+ensures sat(t, eventual(LockedIthPositionWithHigherEpochTemporal(b, i, epoch', config)))
+{
+    reveal_eventual();
+    var tt := eventualStep(t, LockedIthPositionWithEpochTemporal(b, i, epoch, config));
+    assert sat(tt, LockedIthPositionWithHigherEpochTemporal(b, i, epoch', config));
+}
+
+lemma EpochMonotone(b:Behavior<LS_State>, node:EndPoint, t1:int, t2:int, config:Config)
+requires ValidBehavior(b, config)
+requires 0 <= t1 <= t2
+requires node in config
+ensures node in b[t1].servers
+ensures node in b[t2].servers
+ensures b[t1].servers[node].epoch <= b[t2].servers[node].epoch
+{
+    var k := t1;
+    ValidBehaviorServers(b, config);
+    while (k < t2)
+    invariant t1 <= k <= t2
+    invariant b[t1].servers[node].epoch <= b[k].servers[node].epoch
+    {
+        k := k + 1;
+    }
+}
+
+lemma ValidTransferHasLargestEpoch(b:Behavior<LS_State>, t:int, p:LockPacket, config:Config)
+requires ValidBehavior(b, config)
+requires t >= 0
+requires ValidTransferPacket(p, config)
+requires b[t].environment.nextStep.LEnvStepHostIos?
+requires LIoOpSend(p) in b[t].environment.nextStep.ios
+ensures LargestEpoch(b[t], p.msg.transfer_epoch)
+{
+    var lb := MapToSeq(b, t);
+    var glb := LSToGLS(config, lb);
+    var src := p.src;
+    assert src in config;
+    ValidBehaviorServers(b, config);
+
+    assert b[t].servers[src].held;
+    assert glb[t].ls.servers[src].epoch == |glb[t].history|;
+    assert p.msg.transfer_epoch == |glb[t].history| + 1;
+
+    forall s |
+           s in config
+    ensures s in b[t].servers
+    ensures p.msg.transfer_epoch > b[t].servers[s].epoch
+    {
+        ValidBehaviorServers(b, config);
+        if (b[t].servers[s].epoch > 0) {
+            assert p.msg.transfer_epoch > b[t].servers[s].epoch;
+        }
+
+    }
 
 }
 
-// lemma LockedWithEpochToHigherEpoch(b:Behavior<LS_State>, t:int, i:int, epoch:int, epoch':int, config:Config)
-// requires imaptotal(b)
-// requires 0 <= i < |config|
-// requires sat(t, LockedIthPositionWithEpochTemporal(b, i, epoch, config))
-// requires epoch > epoch'
-// ensures sat(t, LockedIthPositionWithHigherEpochTemporal(b, i, epoch', config))
-// {
-// }
 
-// lemma LockEventuallyTransferToNextNode(b:Behavior<LS_State>, i:int, epoch:int, config:Config, asp:AssumptionParameters)
-// requires ValidBehavior(b, config)
-// requires LivenessAssumptions(b, asp, config)
-// requires 0 <= i < |config|
-// ensures sat(0, always(LockTransferToNextNode(b, i, epoch, config)))
-// {
-//     forall t |
-//            t >= 0
-//         && sat(t, or(LockedIthPositionWithEpochTemporal(b, i, epoch, config),
-//                      LockedIthPositionWithHigherEpochTemporal(b, i, epoch, config)))
-//     ensures sat(t, eventual(LockedIthPositionWithHigherEpochTemporal(b, NextNode(i, config), epoch, config)))
-//     {
-//         var e := epoch;
-//         if (sat(t, LockedIthPositionWithHigherEpochTemporal(b, i, epoch, config))) 
-//         {
-//             e := GetEpoch(b, t, i, epoch, config);
-//         }
-//         assert e >= epoch;
-//         assert sat(t, LockedIthPositionWithEpochTemporal(b, i, e, config));
-// 
-//         EventuallyNodeGrant(b, i, e, config, asp);
-//         reveal_always();
-//         reveal_imply();
-//         assert sat(t, eventual(NodeGrantPacketTemporal(b, i, e+1, config)));
-//         var grantStep := eventualStep(t, NodeGrantPacketTemporal(b, i, e+1, config));
-//         var p := GetTransferPacket(b, grantStep, i, e+1, config);
-//         var serverAddresses := MapSeqToSet(config, x=>x);
-//         assert forall x :: x in serverAddresses <==> x in config;
-//         var bEnv := BehaviorToLEnvMap(b);
-//         assert PacketSentBetweenHosts(bEnv[grantStep], p, serverAddresses, serverAddresses);
-//         assert sat(grantStep, PacketsEventuallyDeliveredForHostsTemporal(bEnv, serverAddresses));
-//         assert sat(grantStep, next(eventual(PacketDeliveredTemporal(bEnv, p))));
-//         reveal_next();
-//         reveal_eventual();
-//         assert sat(grantStep, eventual(PacketDeliveredTemporal(bEnv, p)));
-//         var acceptStep := eventualStep(grantStep, PacketDeliveredTemporal(bEnv, p));
-//         TransferDeliveredLeadsToLockedLemma(b, p, NextNode(i, config), config);
-//         assert sat(acceptStep, next(LockedIthPositionWithEpochTemporal(b, NextNode(i, config), e+1, config)));
-//         assert sat(acceptStep+1, LockedIthPositionWithEpochTemporal(b, NextNode(i, config), e+1, config));
-//         LockedWithEpochToHigherEpoch(b, acceptStep+1, NextNode(i, config), e+1, epoch, config);
-//         assert sat(acceptStep+1, LockedIthPositionWithHigherEpochTemporal(b, NextNode(i, config), epoch, config));
-//     }
-//     reveal_always();
-// }
+
+lemma FirstReceiveLeadsToLocked(b:Behavior<LS_State>, t:int, grantT:int, p:LockPacket, i:int, config:Config)
+requires ValidBehavior(b, config)
+requires t >= 0
+requires ValidTransferPacket(p, config)
+requires 0 <= i < |config|
+requires 0 <= grantT < t
+requires p.src in config
+requires p.dst == config[i]
+requires sat(t, PacketReceivedTemporal(b, p))
+requires forall t' :: grantT <= t' < t ==> !sat(t', PacketReceivedTemporal(b, p))
+requires config[i] in b[grantT].servers
+requires !b[grantT+1].servers[config[i]].held
+requires p.msg.transfer_epoch > b[grantT+1].servers[config[i]].epoch
+ensures sat(t, next(LockedIthPositionWithEpochTemporal(b, i, p.msg.transfer_epoch, config)))
+{
+    var ios := b[t].environment.nextStep.ios;
+    var node := config[i];
+    ValidBehaviorServers(b, config);
+    NodeConfig(b, config);
+    assert NodeAccept(b[t].servers[node], b[t+1].servers[node], ios);
+    assert node == b[t].environment.nextStep.actor;
+
+
+    var k := grantT+1;
+    while (k < t)
+    invariant node == config[i]
+    invariant grantT+1 <= k <= t
+    invariant node in b[k].servers
+    invariant !b[k].servers[node].held
+    invariant p.msg.transfer_epoch > b[k].servers[node].epoch
+    {
+        ValidBehaviorServers(b, config);
+        if (b[k].environment.nextStep.LEnvStepHostIos?
+         && b[k].environment.nextStep.actor == node
+         && LS_NextOneServer(b[k], b[k+1], node, b[k].environment.nextStep.ios)
+         && NodeAccept(b[k].servers[node], b[k+1].servers[node], b[k].environment.nextStep.ios)) {
+            
+            var kios := b[k].environment.nextStep.ios;
+            assert |kios| >= 1;
+            if (kios[0].LIoOpReceive?) {
+                if (ValidTransferPacket(kios[0].r, config)) {
+                    var pp := kios[0].r;
+                    assert b[k].environment.nextStep.LEnvStepHostIos?;
+                    assert LIoOpReceive(pp) in b[k].environment.nextStep.ios;
+                    assert PacketReceived(b[k], pp);
+                    assert sat(k, PacketReceivedTemporal(b, pp));
+                    assert ValidTransferPacket(pp, config);
+                    if (pp == p) {
+                        assert sat(k, PacketReceivedTemporal(b, p));
+                    }
+                    assert pp != p;
+                    assert pp.dst == node;
+                    if (pp.msg.transfer_epoch > b[k].servers[node].epoch) {
+                        OnlyOneUsefulTransfer(b, k, p, pp, node, config);
+                        assert pp == p;
+                    }
+                    assert p.msg.transfer_epoch > b[k+1].servers[node].epoch;
+                    assert !b[k+1].servers[node].held;
+                } else {
+                    var pp := kios[0].r;
+                    NodeConfig(b, config);
+                    assert IsValidLIoOp(kios[0], b[k].environment.nextStep.actor, b[k].environment);
+                    assert pp.dst == b[k].environment.nextStep.actor;
+                    assert node in b[k+1].servers;
+                    assert pp.dst == node;
+                    ValidBehaviorServers(b, config);
+                    assert pp.dst in config;
+                    assert !b[k+1].servers[node].held;
+                }
+
+                assert !b[k+1].servers[node].held;
+                assert p.msg.transfer_epoch > b[k+1].servers[node].epoch;
+            }
+        }         
+        k := k + 1;
+    }
+
+
+    assert !b[t].servers[node].held;
+    assert p.msg.transfer_epoch > b[t].servers[node].epoch;
+
+    assert ios[1].LIoOpSend?;
+    var lockedP := ios[1].s;
+    assert lockedP.msg.Locked?;
+    assert IsValidLIoOp(ios[1], b[t].environment.nextStep.actor, b[t].environment);
+    assert lockedP.src == b[t].environment.nextStep.actor;
+    assert lockedP.src == node;
+    assert lockedP.msg.locked_epoch == p.msg.transfer_epoch;
+    assert lockedP in b[t+1].environment.sentPackets;
+
+    assert exists pp ::
+                  pp in b[t+1].environment.sentPackets
+               && pp.src == node
+               && pp.msg.Locked?
+               && pp.msg.locked_epoch == p.msg.transfer_epoch;
+    assert sat(t+1, LockedIthPositionWithEpochTemporal(b, i, p.msg.transfer_epoch, config));
+    reveal_next();
+}
+
+
+
+
+
+lemma LockEventuallyTransferToNextNode(b:Behavior<LS_State>, i:int, epoch:int, config:Config, asp:AssumptionParameters)
+requires ValidBehavior(b, config)
+requires LivenessAssumptions(b, asp, config)
+requires 0 <= i < |config|
+requires epoch < 0xFFFF_FFFF_FFFF_FFFF
+ensures sat(0, always(LockTransferToNextNode(b, i, epoch, config)))
+{
+    forall t |
+           t >= 0
+        && sat(t, LockedIthPositionWithEpochTemporal(b, i, epoch, config))
+    ensures sat(t, eventual(LockedIthPositionWithEpochTemporal(b, NextNode(i, config), epoch+1, config)))
+    {
+        var e := epoch;
+        EventuallyNodeGrant(b, i, e, config, asp);
+        reveal_always();
+        reveal_imply();
+        assert sat(t, eventual(NodeGrantPacketTemporal(b, i, e+1, config)));
+        var eventualGrantStep := eventualStep(t, NodeGrantPacketTemporal(b, i, e+1, config));
+        var p := GetTransferPacket(b, eventualGrantStep, i, e+1, config);
+        var grantStep := GetSendStep(b, eventualGrantStep, p, config);
+        var serverAddresses := MapSeqToSet(config, x=>x);
+        assert forall x :: x in serverAddresses <==> x in config;
+        var bEnv := BehaviorToLEnvMap(b);
+        assert PacketSentBetweenHosts(bEnv[grantStep], p, serverAddresses, serverAddresses);
+        assert sat(grantStep, PacketsEventuallyDeliveredForHostsTemporal(bEnv, serverAddresses));
+        assert sat(grantStep, next(eventual(PacketDeliveredTemporal(bEnv, p))));
+        reveal_next();
+        reveal_eventual();
+        assert sat(grantStep, eventual(PacketDeliveredTemporal(bEnv, p)));
+        var dStep := eventualStep(grantStep, PacketDeliveredTemporal(bEnv, p));
+        lemma_TransferDeliveredLeadsToReceived(b, p, NextNode(i, config), config, asp);
+        assert sat(dStep + 1, eventual(PacketReceivedTemporal(b, p)));
+        assert sat(grantStep, eventual(PacketReceivedTemporal(b, p)));
+        var acceptStep := FirstEventualStep(grantStep, PacketReceivedTemporal(b, p));
+        ValidBehaviorServers(b, config);
+        assert config[NextNode(i, config)] in b[grantStep+1].servers;
+        ValidTransferHasLargestEpoch(b, grantStep, p, config);
+        assert p.msg.transfer_epoch > b[grantStep].servers[config[NextNode(i, config)]].epoch;
+
+        assert b[grantStep].servers[config[i]].held;
+        if (i == NextNode(i, config)) {
+            assert !b[grantStep+1].servers[config[NextNode(i, config)]].held;
+        } else {
+            OneLockedAtMost(b, config);
+            assert !b[grantStep].servers[config[NextNode(i, config)]].held;
+            assert !b[grantStep+1].servers[config[NextNode(i, config)]].held;
+        }
+
+        assert !b[grantStep+1].servers[config[NextNode(i, config)]].held;
+        FirstReceiveLeadsToLocked(b, acceptStep, grantStep, p, NextNode(i, config), config);
+        assert sat(acceptStep, next(LockedIthPositionWithEpochTemporal(b, NextNode(i, config), e+1, config)));
+        assert sat(acceptStep+1, LockedIthPositionWithEpochTemporal(b, NextNode(i, config), e+1, config));
+        assert sat(acceptStep+1, LockedIthPositionWithEpochTemporal(b, NextNode(i, config), e+1, config));
+        if (t <= acceptStep + 1) {
+            assert sat(t, eventual(LockedIthPositionWithEpochTemporal(b, NextNode(i, config), e+1, config)));
+        } else {
+            // var pp :|
+            //     exists epoch' ::
+            //            epoch' > epoch
+            //         && pp in b[acceptStep+1].environment.sentPackets
+            //         && pp.src == config[NextNode(i, config)]
+            //         && pp.msg.Locked?
+            //         && pp.msg.locked_epoch == epoch';
+            // assert pp in b[t+1].environment.sentPackets;
+
+            var pp :|
+                pp in b[acceptStep+1].environment.sentPackets
+             && pp.src == config[NextNode(i, config)]
+             && pp.msg.Locked?
+             && pp.msg.locked_epoch == e+1;
+
+            SentPacketsMonotoneMeta(b, acceptStep+1, config, pp);
+            assert pp in b[t+1].environment.sentPackets;
+
+            assert sat(t+1, LockedIthPositionWithEpochTemporal(b, NextNode(i, config), e+1, config));
+
+            reveal_eventual();
+
+            assert sat(t, eventual(LockedIthPositionWithEpochTemporal(b, NextNode(i, config), e+1, config)));
+        }
+    }
+    reveal_always();
+}
 
 
 
