ironfleet/src/Dafny/Distributed/LockProof/LivenessProof/Misc.i.dfy
@@ -1,0 +1,460 @@
+include "Defs.i.dfy"
+include "Assumptions.i.dfy"
+include "../proof.i.dfy"
+
+module Lock__LivenessProof__Misc_i {
+
+import opened Lock__LivenessProof__Defs_i
+import opened Lock__LivenessProof__Assumptions_i
+import opened LockProof
+
+
+
+lemma ValidBehaviorServers(b:Behavior<LS_State>, config:Config)
+requires ValidBehavior(b, config)
+ensures forall t :: t >= 0 ==> forall i :: i in b[t].servers <==> i in config
+{
+    forall t |
+           t >= 0
+    ensures forall i :: i in b[t].servers <==> i in config
+    {
+        assert forall i :: i in b[0].servers <==> i in config;
+        var k := 0;
+        while (k < t) 
+        invariant 0 <= k <= t
+        invariant forall i :: i in b[k].servers <==> i in config
+        {
+            k := k + 1;
+        }
+    }
+}
+
+lemma FirstEventualStep(step:int, t:temporal) 
+returns (step':int)
+requires sat(step, eventual(t))
+ensures sat(step', t)
+ensures step' >= step
+ensures forall i :: step <= i < step' ==> !sat(i, t)
+{
+    reveal_eventual();
+    var es := eventualStep(step, t);
+    step' := step;
+    while (step' < es)
+    invariant step <= step'
+    invariant forall i :: step <= i < step' ==> !sat(i, t)
+    {
+        if (sat(step', t)) {
+            break;
+        } else {
+            step' := step' + 1;
+        }
+    }
+}
+
+lemma GetLockPacket(ls:LS_State, i:int, epoch:int, config:Config) 
+returns (p:LockPacket)
+requires 0 <= i < |config|
+requires LockedIthPositionWithEpoch(ls, i, epoch, config)
+ensures p in ls.environment.sentPackets
+     && p.src == config[i]
+     && p.msg.Locked?
+     && p.msg.locked_epoch == epoch
+{
+    p :| 
+        p in ls.environment.sentPackets
+     && p.src == config[i]
+     && p.msg.Locked?
+     && p.msg.locked_epoch == epoch;
+}
+
+lemma SentPacketsMonotoneMeta(b:Behavior<LS_State>, t:int, config:Config, p:LockPacket) 
+requires ValidBehavior(b, config)
+requires t >= 0
+requires p in b[t].environment.sentPackets
+ensures forall t' :: t' >= t ==> p in b[t'].environment.sentPackets
+{
+    forall t' |
+           t' >= t
+    ensures p in b[t'].environment.sentPackets
+    {
+        var k := t;
+        while (k < t')
+        invariant t <= k <= t'
+        invariant p in b[k].environment.sentPackets
+        {
+            k := k + 1;
+        }
+    }
+}
+
+lemma GetSendStep(b:Behavior<LS_State>, t:int, p:LockPacket, config:Config)
+returns (t':int)
+requires ValidBehavior(b, config)
+requires t >= 0
+requires p in b[t].environment.sentPackets
+ensures 0 <= t' <= t
+ensures b[t'].environment.nextStep.LEnvStepHostIos?
+ensures LIoOpSend(p) in b[t'].environment.nextStep.ios
+ensures b[t'].environment.nextStep.actor == p.src
+{
+    assert !(p in b[0].environment.sentPackets);
+    var k := 0;
+    while (k < t && !(p in b[k+1].environment.sentPackets))
+    invariant 0 <= k <= t
+    invariant forall i :: 0 <= i <= k ==> !(p in b[i].environment.sentPackets)
+    {
+        k := k + 1;
+    }
+    assert !(p in b[k].environment.sentPackets);
+    assert p in b[k+1].environment.sentPackets;
+    t' := k;
+    assert b[t'].environment.nextStep.LEnvStepHostIos?;
+    assert LIoOpSend(p) in b[t'].environment.nextStep.ios;
+}
+
+lemma SentPacketsMonotone(b:Behavior<LS_State>, t:int, i:int, epoch:int, config:Config)
+requires ValidBehavior(b, config)
+requires t >= 0
+requires 0 <= i < |config|
+requires sat(t, NodeGrantPacketTemporal(b, i, epoch, config))
+ensures forall x :: x >= 0 ==> sat(x, eventual(NodeGrantPacketTemporal(b, i, epoch, config)))
+{
+    assert NodeGrantPacket(b[t], i, epoch, config);
+    var p :|
+        p in b[t].environment.sentPackets
+     && p.src == config[i]
+     && p.dst == config[NextNode(i, config)]
+     && p.msg.Transfer?
+     && p.msg.transfer_epoch == epoch;
+    SentPacketsMonotoneMeta(b, t, config, p);
+    assert forall t' :: t' >= t ==> p in b[t'].environment.sentPackets;
+
+    forall x |
+           x >= 0
+    ensures sat(x, eventual(NodeGrantPacketTemporal(b, i, epoch, config)))
+    {
+        var tt := t + 1;
+        if (tt <= x) {
+            tt := x + 1;
+        }
+        assert tt > x;
+        assert p in b[tt].environment.sentPackets;
+        assert sat(tt, NodeGrantPacketTemporal(b, i, epoch, config));
+        reveal_eventual();
+    }
+}
+
+lemma NodeConfig(b:Behavior<LS_State>, config:Config)
+requires ValidBehavior(b, config)
+ensures forall t, i ::
+               t >= 0
+            && i in b[t].servers
+           ==> b[t].servers[i].config == config
+ensures forall t, i ::
+               t >= 0
+            && 0 <= i < |config|
+           ==> config[i] in b[t].servers 
+            && b[t].servers[config[i]].my_index == i
+{
+    forall t |
+           t >= 0
+    ensures forall i ::
+                   i in b[t].servers
+               ==> b[t].servers[i].config == config
+    {
+        assert forall i :: 
+                      i in b[0].servers
+                  ==> b[0].servers[i].config == config;
+        var k := 0;
+        while (k < t)
+        invariant 0 <= k <= t
+        invariant forall i :: i in b[k].servers ==> b[k].servers[i].config == config
+        {
+            k := k + 1;
+        }
+    }
+
+    forall t | 
+           t >= 0
+    ensures forall i ::
+                   0 <= i < |config|
+               ==> config[i] in b[t].servers
+                && b[t].servers[config[i]].my_index == i
+    {
+        forall i |
+               0 <= i < |config|
+        ensures config[i] in b[0].servers
+             && b[0].servers[config[i]].my_index == i
+        {
+            assert NodeInit(b[0].servers[config[i]], i, config);
+        }
+
+        var k := 0;
+        while (k < t)
+        invariant 0 <= k <= t
+        invariant forall i ::
+                         0 <= i < |config|
+                     ==> config[i] in b[k].servers
+        invariant forall i ::
+                         0 <= i < |config|
+                     ==> b[k].servers[config[i]].my_index == i
+        {
+            assert LS_Next(b[k], b[k+1]);
+
+            if (b[k].environment.nextStep.LEnvStepHostIos?
+             && b[k].environment.nextStep.actor in b[k].servers)
+            {
+                var id := b[k].environment.nextStep.actor;
+                assert forall i :: 0 <= i < |config| && config[i] != id ==> b[k+1].servers[config[i]].my_index == i;
+                assert forall i :: 0 <= i < |config| && config[i] == id ==> b[k+1].servers[config[i]].my_index == i;
+            }
+
+            assert forall i :: 0 <= i < |config| ==> b[k+1].servers[config[i]].my_index == i;
+            k := k + 1;
+        }
+    }
+}
+
+
+
+lemma EventuallyReceiveStep(b:Behavior<LS_State>, node:EndPoint, config:Config, asp:AssumptionParameters)
+requires ValidBehavior(b, config)
+requires node in config
+requires LivenessAssumptions(b, asp, config)
+ensures sat(0, always(eventual(ReceiveStepTemporal(b, node))))
+{
+    reveal_and();
+    reveal_always();
+    assert sat(0, always(ActionOccursForServerTemporal(b, node)));
+    assert sat(0, always(eventual(NodeAcceptOccursForServerTemporal(b, node))));
+    forall t |
+           t >= 0
+    ensures sat(t, eventual(ReceiveStepTemporal(b, node)))
+    {
+        assert sat(t, eventual(NodeAcceptOccursForServerTemporal(b, node)));
+        var t' := eventualStep(t, NodeAcceptOccursForServerTemporal(b, node));
+        assert sat(t', NodeAcceptOccursForServerTemporal(b, node));
+        assert NodeAcceptOccursForServer(b[t'], b[t'+1], node);
+        assert ReceiveStep(b[t'], node);
+        assert sat(t', ReceiveStepTemporal(b, node));
+        reveal_eventual();
+        assert sat(t, eventual(ReceiveStepTemporal(b, node)));
+    }
+}
+
+
+
+lemma HostQueueDecrease(e:LockEnvironment, e':LockEnvironment, p:LockPacket, dst:EndPoint, index:int) 
+returns (index':int)
+requires LEnvironment_Next(e, e')
+requires HostQueues_Next(e, e')
+requires p.dst == dst
+requires p.dst in e.hostInfo
+requires 0 <= index < |e.hostInfo[dst].queue|
+requires p == e.hostInfo[dst].queue[index]
+requires e.nextStep.LEnvStepHostIos?
+requires |e.nextStep.ios| > 0
+requires e.nextStep.ios[0].LIoOpReceive?
+requires HostQueue_PerformIos(e.hostInfo[dst].queue, e'.hostInfo[dst].queue, e.nextStep.ios)
+ensures (index' < index 
+      && 0 <= index' < |e'.hostInfo[dst].queue| 
+      && p == e'.hostInfo[dst].queue[index']) 
+     || (LIoOpReceive(p) in e.nextStep.ios
+      && index' == -1
+      && index' < index)
+{
+    var ios := e.nextStep.ios;
+    var queue := e.hostInfo[dst].queue;
+    var queue' := e'.hostInfo[dst].queue;
+    index' := index;
+    assert HostQueue_PerformIos(queue, queue', ios);
+    if (LIoOpReceive(p) == ios[0]) {
+        index' := -1;
+    } else {
+        ios := ios[1..];
+        queue := queue[1..];
+        index' := index' - 1;
+        assert HostQueue_PerformIos(queue, queue', ios);
+    
+        while (|ios| > 0 && ios[0].LIoOpReceive?)
+        decreases |ios|
+        decreases index'
+        invariant index' < index
+        invariant |ios| >= 0
+        invariant forall x :: x in ios ==> x in e.nextStep.ios
+        invariant -1 <= index' < |queue|
+        invariant index' != -1 ==> p == queue[index']
+        invariant index' == -1 ==> (|ios| > 0 && LIoOpReceive(p) == ios[0])
+        invariant HostQueue_PerformIos(queue, queue', ios)
+        {
+            if (LIoOpReceive(p) == ios[0]) {
+                index' := -1;
+                break;
+            } else {
+                ios := ios[1..];
+                queue := queue[1..];
+                index' := index' - 1;
+            }
+            assert index' < index;
+        }
+        if (index' == -1) {
+            assert LIoOpReceive(p) == ios[0];
+            assert LIoOpReceive(p) in e.nextStep.ios;
+            assert index' < index;
+        } else {
+            assert 0 <= index' < |e'.hostInfo[dst].queue|;
+            assert p == e'.hostInfo[dst].queue[index'];
+            assert index' < index;
+        }
+    }
+}
+
+
+lemma lemma_TransferDeliveredLeadsToReceived(b:Behavior<LS_State>, p:LockPacket, i:int, config:Config, asp:AssumptionParameters)
+requires ValidBehavior(b, config)
+requires LivenessAssumptions(b, asp, config)
+requires p.msg.Transfer?
+requires 0 <= i < |config|
+requires p.dst == config[i]
+ensures sat(0, always(PacketDeliveredLeadsToReceived(b, p)))
+{
+    forall t |
+           t >= 0
+        && sat(t, PacketDeliveredTemporal(BehaviorToLEnvMap(b), p))
+    ensures sat(t+1, eventual(PacketReceivedTemporal(b, p)))
+    {
+        var node := p.dst;
+        reveal_always();
+        assert sat(t, HostQueuesNextTemporal(BehaviorToLEnvMap(b)));
+        assert HostQueues_Next(b[t].environment, b[t+1].environment);
+        assert node in b[t].environment.hostInfo;
+        assert p in b[t+1].environment.hostInfo[node].queue;
+        var index :| 
+            0 <= index < |b[t+1].environment.hostInfo[node].queue|
+         && p == b[t+1].environment.hostInfo[node].queue[index];
+        var k := t+1;
+        while (index >= 0)
+        decreases index
+        invariant k >= t+1
+        invariant node in b[k].environment.hostInfo
+        invariant -1 <= index < |b[k].environment.hostInfo[node].queue|
+        invariant index >= 0 ==> p == b[k].environment.hostInfo[node].queue[index]
+        invariant index == -1  
+              ==> (b[k-1].environment.nextStep.LEnvStepHostIos?
+                && LIoOpReceive(p) in b[k-1].environment.nextStep.ios)
+        {
+            EventuallyReceiveStep(b, node, config, asp);
+            reveal_always();
+            assert sat(k, eventual(ReceiveStepTemporal(b, node)));
+            var rStep := FirstEventualStep(k, ReceiveStepTemporal(b, node));
+
+            var kk := k;
+            while (kk < rStep)
+            invariant k <= kk <= rStep
+            invariant node in b[kk].environment.hostInfo
+            invariant 0 <= index < |b[kk].environment.hostInfo[node].queue|
+            invariant p == b[kk].environment.hostInfo[node].queue[index]
+            {
+                assert sat(kk, HostQueuesNextTemporal(BehaviorToLEnvMap(b)));
+                if (b[kk].environment.nextStep.LEnvStepHostIos?) {
+                    assert !sat(kk, ReceiveStepTemporal(b, node));
+                    assert !ReceiveStep(b[kk], node);
+                    assert node in b[kk+1].environment.hostInfo;
+                    assert 0 <= index < |b[kk+1].environment.hostInfo[node].queue|;
+                    assert p == b[kk+1].environment.hostInfo[node].queue[index];
+
+                }
+
+                kk := kk + 1;
+            }
+
+            assert sat(rStep, HostQueuesNextTemporal(BehaviorToLEnvMap(b)));
+            var index' := HostQueueDecrease(b[rStep].environment, b[rStep+1].environment, p, node, index);
+
+            assert index' < index;
+            index := index';
+            k := rStep + 1;
+
+        }
+
+        assert sat(k-1, PacketReceivedTemporal(b, p));
+        assert k-1 >= t+1;
+        reveal_eventual();
+        assert sat(t+1, eventual(PacketReceivedTemporal(b, p)));
+    }
+
+    reveal_always();
+    reveal_imply();
+    reveal_next();
+}
+
+lemma MapToSeq(b:Behavior<LS_State>, t:int) 
+returns (lb:seq<LS_State>)
+requires t >= 0
+requires imaptotal(b)
+ensures |lb| == t + 1
+ensures forall i :: 0 <= i <= t ==> lb[i] == b[i]
+{
+    lb := [b[0]];
+    var k := 0;
+    while (k < t)
+    invariant 0 <= k <= t
+    invariant |lb| == k + 1
+    invariant forall i :: 0 <= i <= k ==> lb[i] == b[i]
+    {
+        lb := lb + [b[k+1]];
+        k := k + 1;
+    }
+}
+
+lemma OneLockedAtMost(b:Behavior<LS_State>, config:Config)
+requires ValidBehavior(b, config)
+ensures forall t ::
+               t >= 0
+           ==> forall x :: x in config <==> x in b[t].servers
+ensures forall t ::
+               t >= 0
+           ==> (exists id ::
+                       id in config
+                    && forall x ::
+                              x in config
+                          ==> (b[t].servers[x].held <==> x == id))
+            || ((forall id ::
+                        id in config
+                    ==> !b[t].servers[id].held))
+{
+    ValidBehaviorServers(b, config);
+    forall t |
+           t >= 0
+    ensures (exists id ::
+                    id in config
+                 && forall x :: 
+                           x in config
+                       ==> (b[t].servers[x].held <==> x == id))
+         || ((forall id ::
+                     id in config
+                 ==> !b[t].servers[id].held))
+    {
+        var lb := MapToSeq(b, t);
+        var glb := LSToGLS(config, lb);
+        assert Less_Than_One_Hold(glb[t]);
+        var gls := glb[t];
+        assert (forall s ::
+                       s in glb[t].ls.servers
+                   ==> (s == gls.history[|gls.history|-1] <==> gls.ls.servers[s].held))
+            || (forall s :: s in gls.ls.servers ==> !gls.ls.servers[s].held);
+        ValidBehaviorServers(b, config);
+        assert gls.ls == lb[t];
+        assert gls.history[|gls.history|-1] in config;
+        assert (forall s ::
+                       s in config
+                   ==> (s == gls.history[|gls.history|-1] <==> gls.ls.servers[s].held))
+            || (forall s :: s in gls.ls.servers ==> !gls.ls.servers[s].held);
+        assert (forall s ::
+                       s in config
+                   ==> (s == gls.history[|gls.history|-1] <==> lb[t].servers[s].held))
+            || (forall s :: s in config ==> !lb[t].servers[s].held);
+    }
+}
+
+}
